In SHA256.v, the "functional specification" had really been, all along, not a functional spec but an efficient functional program.  As such it was not so well suited for the verification of the C program.  With this check-in, SHA256 is divided into two parts: 1. Functional spec.  It's more elegant, but it takes  exponential time to compute (for same reason that recursive  fibonacci program takes exponential time). 2. Functional program (computes inside Coq only 10^4 times slow   than the C program). Then, in sha_lemmas2.v, these two functional programs are proved   equal.  Most (or all?) of the C program proof is now with respect to   the functional spec, not the functional program.

sha/SHA256.v
@@ -1,17 +1,38 @@
-(*Stephen Yi-Hsien Lin 05/15/2013,  modified by Andrew Appel, October 2013 *)
+(* Andrew W. Appel and Stephen Yi-Hsien Lin,
+    May 2013, October 2013, March 2014 *)
 
 Require Recdef.
 Require Import Integers.
 Require Import Coqlib.
 Require Import Coq.Strings.String.
 Require Import Coq.Strings.Ascii.
+Require Import List. 
 
 Notation "[ ]" := nil.
 Notation "[ x , .. , y ]" := (cons x .. (cons y []) ..).
 
+Lemma skipn_length:
+  forall {A} n (al: list A), 
+    (length al >= n)%nat -> 
+    (length (skipn n al) = length al - n)%nat.
+Proof.
+ induction n; destruct al; simpl; intros; auto.
+ apply IHn. omega.
+Qed.
+
+Lemma skipn_length_short:
+  forall {A} n (al: list A), 
+    (length al < n)%nat -> 
+    (length (skipn n al) = 0)%nat.
+Proof.
+ induction n; destruct al; simpl; intros; auto.
+ omega.
+ apply IHn. omega.
+Qed.
+
 (* PREPROCESSING: CONVERTING STRINGS TO PADDED MESSAGE BLOCKS *)
 
-(*converting a string to a list of N*)
+(*converting a string to a list of Z *)
 Fixpoint str_to_Z (str : string) : list Z :=
   match str with
     |EmptyString => nil
@@ -22,15 +43,6 @@ Fixpoint str_to_Z (str : string) : list Z :=
 Definition Z_to_Int (a b c d : Z) : Int.int :=
   Int.or (Int.or (Int.or (Int.shl (Int.repr a) (Int.repr 24)) (Int.shl (Int.repr b) (Int.repr 16)))
             (Int.shl (Int.repr c) (Int.repr 8))) (Int.repr d).
-
-Function zeros (n : Z) {measure Z.to_nat n} : list Int.int :=
- if Z.gtb n 0 then Int.zero :: zeros (n-1) else nil.
-Proof.
-   intros. rewrite Z2Nat.inj_sub by omega.
-   apply Zgt_is_gt_bool in teq.
-   assert (0 < n) by omega. apply Z2Nat.inj_lt in H; try omega.
-   simpl in H. change (Z.to_nat 1) with 1%nat. omega.
-Defined.
 
 Fixpoint Zlist_to_intlist (nl: list Z) : list int :=
   match nl with
@@ -43,21 +55,6 @@ Definition generate_and_pad msg :=
    Zlist_to_intlist (msg ++ [128%Z] 
                 ++ list_repeat (Z.to_nat (-(n + 9) mod 64)) 0)
            ++ [Int.repr (n * 8 / Int.modulus), Int.repr (n * 8)].
-
-(* FUNCTIONS USED ONLY FOR DEBUGGING AND TESTING *)
-Definition hexdigit(a: Z) : Z :=
- if Z.leb 48 a && Z.ltb a 58 then Z.sub a 48
- else if Z.leb 65 a && Z.ltb a 71 then Z.sub a 55
- else if Z.leb 97 a && Z.ltb a 103 then Z.sub a 87
- else 0%Z.
-
-Fixpoint hexstring_to_Zlist (s: string): list Z  :=
- match s with
- | String a (String b r) =>  (hexdigit (Z.of_N (N_of_ascii a)) * 16 
-                                         + hexdigit (Z.of_N (N_of_ascii b)))
-                                          :: hexstring_to_Zlist r
- | _ => nil
- end.
 
 (*ROUND FUNCTION*)
 
@@ -87,41 +84,33 @@ Definition Ch (x y z : int) : int :=
 Definition Maj (x y z : int) : int :=
   Int.xor (Int.xor (Int.and x z) (Int.and y z) ) (Int.and x y).
 
-Definition Sh b x := Int.ror x (Int.repr b).
-Definition Rt b x := Int.shru x (Int.repr b).
+Definition Rotr b x := Int.ror x (Int.repr b).
+Definition Shr b x := Int.shru x (Int.repr b).
 
-Definition Sigma_0 (x : int) : int := Int.xor (Int.xor (Sh 2 x) (Sh 13 x)) (Sh 22 x).
-Definition Sigma_1 (x : int) : int := Int.xor (Int.xor (Sh 6 x) (Sh 11 x)) (Sh 25 x).
-Definition sigma_0 (x : int) : int := Int.xor (Int.xor (Sh 7 x) (Sh 18 x)) (Rt 3 x).
-Definition sigma_1 (x : int) : int := Int.xor (Int.xor (Sh 17 x) (Sh 19 x)) (Rt 10 x).
+Definition Sigma_0 (x : int) : int := 
+          Int.xor (Int.xor (Rotr 2 x) (Rotr 13 x)) (Rotr 22 x).
+Definition Sigma_1 (x : int) : int := 
+          Int.xor (Int.xor (Rotr 6 x) (Rotr 11 x)) (Rotr 25 x).
+Definition sigma_0 (x : int) : int := 
+          Int.xor (Int.xor (Rotr 7 x) (Rotr 18 x)) (Shr 3 x).
+Definition sigma_1 (x : int) : int := 
+          Int.xor (Int.xor (Rotr 17 x) (Rotr 19 x)) (Shr 10 x).
 
-(*word function*)
-Definition W (msg : list int) : int :=
- match msg with
- | x0::x1::x2::x3::x4::x5::x6::x7::x8::x9::x10::x11::x12::x13::x14::x15::_ =>
-   (Int.add (Int.add (sigma_1 x1) x6) (Int.add (sigma_0 x14) x15))
- | _ => Int.zero  (* impossible *)
- end.
-
-(*generating 64 words for the given message block imput*)
-Fixpoint generate_word (msg : list int) (n : nat) {struct n}: list int :=
-  match n with
-  |O   => msg 
-  |S n' => generate_word (W msg :: msg) n'
-  end.
-Arguments generate_word msg n : simpl never.
-Global Opaque generate_word. (* for some reason the Arguments...simpl-never
-   command does not do the job *)
-
+(* word function *)
+Function W (M: Z -> int) (t: Z) {measure Z.to_nat t} : int :=
+  if zlt t 16 
+  then M t 
+  else  (Int.add (Int.add (sigma_1 (W M (t-2))) (W M (t-7)))
+               (Int.add (sigma_0 (W M (t-15))) (W M (t-16)))).
+Proof.
+intros; apply Z2Nat.inj_lt; omega.
+intros; apply Z2Nat.inj_lt; omega.
+intros; apply Z2Nat.inj_lt; omega.
+intros; apply Z2Nat.inj_lt; omega.
+Qed.
 
 (*registers that represent intermediate and final hash values*)
 Definition registers := list int.
-
-(*initializing the values of registers, first thirty-two bits of the fractional
-    parts of the square roots of the first eight prime numbers*)
-Definition init_registers : registers := 
-  map Int.repr  [1779033703, 3144134277, 1013904242, 2773480762,
-                        1359893119, 2600822924, 528734635, 1541459225].
 
 Fixpoint map2 {A B C: Type} (f: A -> B -> C) (al: list A) (bl: list B) : list C :=
  match al, bl with
@@ -129,17 +118,107 @@ Fixpoint map2 {A B C: Type} (f: A -> B -> C) (al: list A) (bl: list B) : list C 
   | _, _ => nil
   end.
 
-Definition registers_add: registers -> registers -> registers := map2 Int.add.
+(*initializing the values of registers, first thirty-two bits of the fractional
+    parts of the square roots of the first eight prime numbers*)
+Definition init_registers : registers := 
+  map Int.repr  [1779033703, 3144134277, 1013904242, 2773480762,
+                        1359893119, 2600822924, 528734635, 1541459225].
+
+Definition nthi (il: list int) (t: Z) := nth (Z.to_nat t) il Int.zero.
+
+Function Round  (regs: registers) (M: Z ->int) (t: Z) 
+        {measure (fun t => Z.to_nat(t+1)) t} : registers :=
+ if zlt t 0 then regs 
+ else match Round regs M (t-1) with
+  | [a,b,c,d,e,f,g,h] => 
+     let T1 := Int.add (Int.add (Int.add (Int.add h (Sigma_1 e)) (Ch e f g)) (nthi K t)) (W M t) in
+     let T2 := Int.add (Sigma_0 a) (Maj a b c) in
+       [Int.add T1 T2, a, b, c, Int.add d T1, e, f, g]
+  | _ => nil
+  end.
+Proof. intros; apply Z2Nat.inj_lt; omega.
+Qed.
+
+Definition hash_block (r: registers) (block: list int) : registers :=
+      map2 Int.add r (Round r (nthi block) 63).
+
+Function hash_blocks (r: registers) (msg: list int) {measure length msg} : registers :=
+  match msg with
+  | nil => r
+  | _ => hash_blocks (hash_block r (firstn 16 msg)) (skipn 16 msg)
+  end.
+Proof. intros.
+ destruct (lt_dec (length msg) 16).
+ rewrite skipn_length_short. simpl; omega. rewrite <- teq; auto.
+ rewrite skipn_length. simpl; omega. rewrite <- teq; omega.
+Qed.
+
+Fixpoint intlist_to_Zlist (l: list int) : list Z :=
+ match l with
+ | nil => nil
+ | i::r =>
+     Int.unsigned (Shr 24 i) ::
+     Int.unsigned (Int.and (Shr 16 i) (Int.repr 255)) ::
+     Int.unsigned (Int.and (Shr 8 i) (Int.repr 255)) ::
+     Int.unsigned (Int.and i (Int.repr 255)) ::
+     intlist_to_Zlist r
+ end.
+
+Definition SHA_256 (str : list Z) : list Z :=
+    intlist_to_Zlist (hash_blocks init_registers (generate_and_pad str)).
+
+(* FAST FUNCTIONAL VERSION OF SHA256 *)
+Function zeros (n : Z) {measure Z.to_nat n} : list Int.int :=
+ if Z.gtb n 0 then Int.zero :: zeros (n-1) else nil.
+Proof.
+   intros. rewrite Z2Nat.inj_sub by omega.
+   apply Zgt_is_gt_bool in teq.
+   assert (0 < n) by omega. apply Z2Nat.inj_lt in H; try omega.
+   simpl in H. change (Z.to_nat 1) with 1%nat. omega.
+Defined.
+
+Definition padlen (n: Z) : list Int.int :=
+    let p := n/4+3 (* number of words with trailing 128-byte, 
+                                                      up to 3 zero bytes, and 2 length words *)
+    in let q := (p+15)/16*16 - p   (* number of zero-pad words *)
+      in zeros q ++ [Int.repr (n * 8 / Int.modulus), Int.repr (n * 8)].
+
+Fixpoint generate_and_pad' (n: list Z) len : list Int.int :=
+  match n with
+  | nil => Z_to_Int 128 0 0 0 :: padlen len
+  | [h1]=> Z_to_Int h1 128 0 0 :: padlen (len+1)
+  | [h1, h2] => Z_to_Int h1 h2 128 0 :: padlen (len+2)
+  | [h1, h2, h3] => Z_to_Int h1 h2 h3 128 :: padlen (len+3)
+  | h1::h2::h3::h4::t => Z_to_Int h1 h2 h3 h4 :: generate_and_pad' t (len+4)
+  end.
+
+Definition generate_and_pad_alt (n: list Z) : list Int.int :=
+   generate_and_pad' n 0.
+
+Definition Wnext (msg : list int) : int :=
+ match msg with
+ | x1::x2::x3::x4::x5::x6::x7::x8::x9::x10::x11::x12::x13::x14::x15::x16::_ =>
+   (Int.add (Int.add (sigma_1 x2) x7) (Int.add (sigma_0 x15) x16))
+ | _ => Int.zero  (* impossible *)
+ end.
+
+(*generating 64 words for the given message block imput*)
+Fixpoint generate_word (msg : list int) (n : nat) {struct n}: list int :=
+  match n with
+  |O   => msg 
+  |S n' => generate_word (Wnext msg :: msg) n'
+  end.
+Arguments generate_word msg n : simpl never.
+Global Opaque generate_word. (* for some reason the Arguments...simpl-never
+   command does not do the job *)
 
 (*round function*)
 Definition rnd_function (x : registers) (k : int) (w : int) : registers:=
   match x with 
   |  [a, b, c, d, e, f, g, h] => 
-    [Int.add (Int.add (Int.add (Int.add (Int.add h (Sigma_1 e)) (Ch e f g)) k) w)
-                        (Int.add (Sigma_0 a) (Maj a b c)),
-     a, b, c,
-     Int.add (d) (Int.add (Int.add (Int.add (Int.add h (Sigma_1 e)) (Ch e f g)) k) w),
-     e, f, g]
+     let T1 := Int.add (Int.add (Int.add (Int.add h (Sigma_1 e)) (Ch e f g)) k) w in
+     let T2 := Int.add (Sigma_0 a) (Maj a b c) in
+       [Int.add T1 T2, a, b, c, Int.add d T1, e, f, g]
   | _ => nil  (* impossible *)
   end.
 
@@ -152,7 +231,7 @@ Fixpoint rnd_64 (x: registers) (k w : list int) : registers :=
 Arguments rnd_64  x k w : simpl never.  (* blows up otherwise *)
 
 Definition process_block (r: registers) (block: list int) : registers :=
-       (registers_add r (rnd_64 r K (rev(generate_word block 48)))).
+       (map2 Int.add r (rnd_64 r K (rev(generate_word block 48)))).
 
 Fixpoint grab_and_process_block (n: nat) (r: registers) (firstrev msg: list int) : registers * list int :=
  match n, msg with
@@ -164,7 +243,7 @@ Fixpoint grab_and_process_block (n: nat) (r: registers) (firstrev msg: list int)
 (*iterate through all the message blocks; this could have been done with just a Fixpoint
   if we incorporated grab_and_process_block into process_msg, but I wanted to 
   modularize a bit more. *)
-Function process_msg  (r: registers) (msg : list int) {measure List.length msg}  : registers :=
+Function process_msg  (r: registers) (msg : list int) {measure length msg}  : registers :=
  match msg with
  | nil => r
  | _ => let (r', msg') := grab_and_process_block 16 r nil msg
@@ -183,21 +262,8 @@ Proof.
   omega.
 Defined.
 
-(*wrapping up everything*)
-
-Fixpoint intlist_to_Zlist (l: list int) : list Z :=
- match l with
- | nil => nil
- | i::r =>
-     Int.unsigned (Rt 24 i) ::
-     Int.unsigned (Int.and (Rt 16 i) (Int.repr 255)) ::
-     Int.unsigned (Int.and (Rt 8 i) (Int.repr 255)) ::
-     Int.unsigned (Int.and i (Int.repr 255)) ::
-     intlist_to_Zlist r
- end.
-
-Definition SHA_256 (str : list Z) : list Z :=
-    intlist_to_Zlist (process_msg init_registers (generate_and_pad str)).
+Definition SHA_256' (str : list Z) : list Z :=
+    intlist_to_Zlist (process_msg init_registers (generate_and_pad_alt str)).
 
 (*EXAMPLES*)
 
@@ -208,8 +274,22 @@ Fixpoint listZ_eq (al bl: list Z) : bool :=
  | _, _ => false
   end.
 
+Definition hexdigit(a: Z) : Z :=
+ if Z.leb 48 a && Z.ltb a 58 then Z.sub a 48
+ else if Z.leb 65 a && Z.ltb a 71 then Z.sub a 55
+ else if Z.leb 97 a && Z.ltb a 103 then Z.sub a 87
+ else 0%Z.
+
+Fixpoint hexstring_to_Zlist (s: string): list Z  :=
+ match s with
+ | String a (String b r) =>  (hexdigit (Z.of_N (N_of_ascii a)) * 16 
+                                         + hexdigit (Z.of_N (N_of_ascii b)))
+                                          :: hexstring_to_Zlist r
+ | _ => nil
+ end.
+
 Definition check m h := 
-  listZ_eq (SHA_256 (str_to_Z m)) (hexstring_to_Zlist h) = true.
+  listZ_eq (SHA_256' (str_to_Z m)) (hexstring_to_Zlist h) = true.
 
 (*This input message is 344 bits long, which would have one message block after padding*)
 Goal  check   "The quick brown fox jumps over the lazy dog"
@@ -220,24 +300,4 @@ Proof. vm_compute; auto. Qed.
 Goal check "The Secure Hash Algorithm is a family of cryptographic hash functions published by the National Institute of Standards and Technology (NIST) as a U.S. Federal Information Processing Standard (FIPS)"
  "27c3971526f07a22decc4dc01340c6c4b972ba6d31b74fb1fbb2edf2bce5fea6".
 Proof. vm_compute; auto. Qed.
-
-(* Alternate, faster implementation of generate_and_pad,
-  proved equivalent. *)
-Definition padlen (n: Z) : list Int.int :=
-    let p := n/4+3 (* number of words with trailing 128-byte, 
-                                                      up to 3 zero bytes, and 2 length words *)
-    in let q := (p+15)/16*16 - p   (* number of zero-pad words *)
-      in zeros q ++ [Int.repr (n * 8 / Int.modulus), Int.repr (n * 8)].
-
-Fixpoint generate_and_pad' (n: list Z) len : list Int.int :=
-  match n with
-  | nil => Z_to_Int 128 0 0 0 :: padlen len
-  | [h1]=> Z_to_Int h1 128 0 0 :: padlen (len+1)
-  | [h1, h2] => Z_to_Int h1 h2 128 0 :: padlen (len+2)
-  | [h1, h2, h3] => Z_to_Int h1 h2 h3 128 :: padlen (len+3)
-  | h1::h2::h3::h4::t => Z_to_Int h1 h2 h3 h4 :: generate_and_pad' t (len+4)
-  end.
-
-Definition generate_and_pad_alt (n: list Z) : list Int.int :=
-   generate_and_pad' n 0.
 
