sha/bdo_lemmas.v
@@ -2,89 +2,7 @@ Require Import proofauto.
 Require Import sha.SHA256.
 Require Import sha.spec_sha.
 Require Import sha.sha_lemmas.
-
-Transparent generate_word.
-
-Lemma generate_word_lemma1:
-  forall b n, length b = LBLOCK ->
-   firstn LBLOCK (rev (generate_word (rev b) n)) = b.
-Proof.
-intros.
-change (rev b) with (nil ++ rev b).
-forget (@nil int) as a.
-revert a; induction n; intro.
-unfold generate_word.
-rewrite rev_app_distr.
-rewrite rev_involutive.
-rewrite firstn_app1 by omega.
-rewrite firstn_same; auto; omega.
-unfold generate_word; fold generate_word.
-change (W (a ++ rev b) :: a ++ rev b) with 
-      ((W (a ++ rev b) ::a) ++ rev b).
-apply IHn.
-Qed.
-
-Lemma length_generate_word: forall b n,
-  length (generate_word b n) = (length b + n)%nat.
-Proof.
-Transparent generate_word.
-intros.
-revert b; induction n; intros; simpl.
-unfold generate_word; fold generate_word.
-omega.
-unfold generate_word; fold generate_word.
-rewrite IHn.
-simpl. omega.
-Qed.
-
-Lemma and_mod_15_lem:
- forall (n: Z), 0 <= Int.signed (Int.and (Int.repr n) (Int.repr 15)) < 16.
-Proof.
-intro n.
-unfold Int.and.
-rewrite (Int.unsigned_repr 15) by repable_signed.
-change 15 with (Z.ones 4).
-assert (0 <= Z.land (Int.unsigned (Int.repr n)) (Z.ones 4) < 16).
-rewrite Z.land_ones.
-apply Z.mod_bound_pos. 
-apply Int.unsigned_range. clear; omega. clear; omega.
-rewrite Int.signed_repr; auto.
-repable_signed.
-Qed.
-
-Lemma nth_generate_word_S:
-  forall k i n b', 
-   nth (i+k) (generate_word b' (n+k)) = nth i (generate_word b' n).
-Proof.
-induction k; intros.
-repeat rewrite plus_0_r. auto.
-replace (n + S k)%nat with (S (n + k))%nat by omega.
-unfold generate_word; fold generate_word.
-replace (i + S k)%nat with (S i + k)%nat by omega.
-rewrite IHk by (simpl; omega).
-clear IHk.
-revert i b' ; induction n; intros.
-unfold generate_word; fold generate_word.
-extensionality d; reflexivity.
-unfold generate_word; fold generate_word.
-apply IHn.
-Qed.
-
-Lemma generate_word_small:
-  forall i b n,
-           length b = 16%nat ->
-           (i < length b)%nat -> 
-           nth i (rev (generate_word (rev b) n)) = nth i b.
-Proof.
-intros.
-extensionality d.
-rewrite <- (nth_firstn_low _ _ LBLOCK).
-rewrite (generate_word_lemma1 b n H).
-auto.
-rewrite rev_length, length_generate_word, rev_length, H.
-change LBLOCK with 16%nat. omega.
-Qed.
-Opaque generate_word.
+Require Import sha.sha_lemmas2.
 
 Definition Xarray (b: list int) (i j: Z) :=
    tuints (rev (generate_word (rev b) 48)) (i-16+(j-i) mod 16).
@@ -136,9 +54,6 @@ unfold Xarray, tuints,ZnthV.
  apply Z2Nat.inj_lt; omega.
 Qed.
 
-Definition nthB (b: list int) (i: nat) (n: Z) :=
-  nth (Z.to_nat (Z.of_nat i - 16 + n)) (rev (generate_word (rev b) 48)) Int.zero.
-
 
 Lemma extract_from_b:
   forall b i n,
@@ -179,110 +94,6 @@ Qed.
 
 Definition c64 := 64%nat.  Global Opaque c64.
 Definition c48 := 48%nat.  Global Opaque c48.
-
-
-Transparent generate_word.
-Lemma generate_word_plus:
-  forall msg a b, (16 <= length msg)%nat ->
-         generate_word msg (a+b) = generate_word (generate_word msg a) b.
-Proof.
-intros msg a b.
-revert msg b; induction a; simpl; intros.
-unfold generate_word; fold generate_word.
-auto.
-unfold generate_word; fold generate_word.
-rewrite IHa by (simpl; omega).
-auto.
-Qed.
-
-Lemma nth_rev_generate_word:
- forall i b,
-   length b = LBLOCK -> 
-   (LBLOCK <= i < 64)%nat ->
-    nth i (rev (generate_word (rev b) 48)) Int.zero =
-  Int.add (nthB b i 0)
-    (Int.add (Int.add (sigma_0 (nthB b i 1)) (sigma_1 (nthB b i 14)))
-       (nthB b i 9)).
-Proof.
-intros.
-unfold nthB.
-rewrite <- rev_length in H.
-forget (rev b) as b'.
-clear b.
-change LBLOCK with 16%nat in *.
-assert (length (generate_word b' 48) = 64)%nat 
- by (rewrite length_generate_word, H; reflexivity).
-rewrite rev_nth by omega.
-repeat rewrite rev_nth
- by (rewrite H1; change 64%nat with (Z.to_nat 64); apply Z2Nat.inj_lt; omega).
-rewrite H1.
-rewrite <- (plus_0_l (64 - S i)).
-assert (48 = (i - 16) + 1 + (64 - S i))%nat by (clear - H0; omega).
-rewrite H2 at 2.
-rewrite nth_generate_word_S.
-rewrite generate_word_plus by omega.
-unfold generate_word at 1. 
-unfold nth at 1.
-assert (forall n:nat, (n < 16) ->
-    ((64 - S (Z.to_nat (Z.of_nat i - 16 + Z.of_nat n))) =
-      (16-n) + (48 - S (Z.to_nat (Z.of_nat i - 16)))))%nat.
-clear - H0.
-intros.
-rewrite Z2Nat.inj_add by omega.
-rewrite Nat2Z.id.
-rewrite Z2Nat.inj_sub by omega.
-rewrite Nat2Z.id.
-change (Z.to_nat 16) with 16%nat.
-omega.
-change 0%Z with (Z.of_nat 0); rewrite H3 by (clear; omega).
-change 1%Z with (Z.of_nat 1); rewrite H3 by (clear; omega).
-change 14%Z with (Z.of_nat 14); rewrite H3 by (clear; omega).
-change 9%Z with (Z.of_nat 9); rewrite H3 by (clear; omega).
-clear H3.
-assert (48 = S (Z.to_nat (Z.of_nat i - 16)) + (48 - S (Z.to_nat (Z.of_nat i - 16))))%nat.
-clear - H0.
-rewrite Z2Nat.inj_sub by omega.
-rewrite Nat2Z.id.
-change (Z.to_nat 16) with 16%nat.
-omega.
-pattern (generate_word b' 48).
-rewrite H3 at 1.
-repeat rewrite nth_generate_word_S.
-rewrite Z2Nat.inj_sub by omega.
-rewrite Nat2Z.id.
-change (Z.to_nat 16) with 16%nat.
-simpl.
-change (nth 16) with (@nth int (15+1)).
-change (nth 15) with (@nth int (14+1)).
-change (nth 2) with (@nth int (1+1)).
-change (nth 7) with (@nth int (6+1)).
-replace (S (i-16)) with ((i-16)+1)%nat by omega.
-repeat rewrite nth_generate_word_S.
-assert (length (generate_word b' (i-16)) >= 16)%nat.
-rewrite length_generate_word, H; omega.
-clear - H4.
-forget (generate_word b' (i-16)) as s.
-rename H4 into H.
-do 16 (destruct s; [simpl in H; omega | ]).
-simpl.
-rewrite <- Int.add_assoc.
-rewrite Int.add_commut.
-f_equal.
-rewrite Int.add_commut.
-rewrite <- Int.add_assoc.
-auto.
-Qed.
-
-Opaque generate_word.
-
-Lemma nth_error_nth:
-  forall A (d: A) i al, (i < length al)%nat -> nth_error al i = Some (nth i al d).
-Proof.
-induction i; destruct al; simpl; intros; auto.
-inv H.
-inv H.
-apply IHi; omega.
-Qed.
 
 Lemma Xarray_update:
  forall i bb,
