sha/verif_sha_bdo2.v
@@ -2,6 +2,7 @@ Require Import floyd.proofauto.
 Require Import sha.sha.
 Require Import sha.SHA256.
 Require Import sha.sha_lemmas.
+Require Import sha.sha_lemmas2.
 Require Import sha.spec_sha.
 Local Open Scope logic.
 
@@ -10,33 +11,37 @@ Lemma sha256_block_data_order_return:
             (sh : share) (regs : registers),
   length b = LBLOCK ->
   NPeano.divide LBLOCK (length hashed) ->
-  regs = process_msg init_registers hashed ->
+  regs = hash_blocks init_registers hashed ->
   semax (initialized _t Delta_loop1)
   (PROP  ()
    LOCAL  (`(eq ctx) (eval_id _ctx))
    SEP 
    (`(array_at tuint Tsh
-        (tuints
-           (map2 Int.add regs
-              (rnd_64 regs K (rev (generate_word (rev b) 48))))) 0 8 ctx);
+        (tuints (hash_block regs b)) 0 8 ctx);
    K_vector;
    `(array_at_ tuint Tsh 0 16) (eval_var _X (tarray tuint 16));
    `(data_block sh (intlist_to_Zlist b) data))) (Sreturn None)
   (frame_ret_assert
      (function_body_ret_assert tvoid
         (`(array_at tuint Tsh
-             (tuints (process_msg init_registers (hashed ++ b))) 0 8 ctx) *
+             (tuints (hash_blocks init_registers (hashed ++ b))) 0 8 ctx) *
          `(data_block sh (intlist_to_Zlist b) data) *
          K_vector))
      (stackframe_of f_sha256_block_data_order)).
 Proof.
 intros.
+assert (H0': (16 | Zlength hashed))
+ by (apply divide_hashed; auto).
+rewrite <- process_block_hash_block. (* FIXME to avoid using process_block at all *)
+2: rewrite H1; apply length_hash_blocks; auto.
+2: assumption.
+unfold process_block.
 unfold Delta_loop1; simplify_Delta.
 forward. (* return; *)
 unfold frame_ret_assert; simpl.
 unfold sha256state_.
-set (regs := map2 Int.add (process_msg init_registers hashed)
-        (rnd_64 (process_msg init_registers hashed) K
+set (regs := map2 Int.add (hash_blocks init_registers hashed)
+        (rnd_64 (hash_blocks init_registers hashed) K
            (rev (generate_word (rev b) 48)))).
 unfold K_vector; unfold_lift.
 erewrite elim_globals_only by (split3; [eassumption | reflexivity.. ]).
@@ -50,5 +55,13 @@ cancel.
 apply derives_refl'; f_equal.
 f_equal.
 unfold regs.
+rewrite <- process_msg_hash_blocks; auto.
+rewrite <- process_msg_hash_blocks; auto.
 apply process_msg_block; auto.
+rewrite initial_world.Zlength_app.
+clear - H0' H.
+destruct H0' as [n ?]; exists (n+1).
+rewrite Z.mul_add_distr_r.
+f_equal; auto.
+rewrite Zlength_correct, H. reflexivity.
 Qed.
