sha/verif_sha_init.v
@@ -35,6 +35,7 @@ apply exp_right with (map Vint init_registers,
 simpl_data_at.
 unfold s256_h, s256_Nh,s256_Nl, s256_num, s256_data, fst,snd.
 entailer!.
+rewrite hash_blocks_equation. reflexivity.
 exists Int.zero, Int.zero; repeat split; reflexivity.
 simpl; change CBLOCK with 64; omega.
 exists 0; simpl; reflexivity.
